wip

Foundation/Modal/Hilbert/KP.lean
@@ -2,38 +2,39 @@ import Foundation.Modal.Hilbert.WellKnown
 import Foundation.Modal.Entailment.KD
 import Foundation.Modal.Entailment.KP
 
-namespace LO.Modal.Hilbert
+namespace LO.Modal
 
 variable {H : Hilbert α}
 
-open Deduction
+namespace Hilbert
 
-section
+open Deduction
 
 class HasP (H : Hilbert α) where
   mem_P : Axioms.P ∈ H.axioms := by tauto;
 
-instance [DecidableEq α] [hP : H.HasP] : Entailment.HasAxiomP H where
+instance [DecidableEq α] [H.HasP] : Entailment.HasAxiomP H.logic where
   P := by
+    constructor;
     apply maxm;
     use Axioms.P;
     constructor;
-    . exact hP.mem_P;
-    . use (.id); simp;
+    . exact HasP.mem_P;
+    . use (.id);
+      simp;
 
-end
+end Hilbert
 
-protected abbrev KP : Hilbert ℕ := ⟨{Axioms.K (.atom 0) (.atom 1), Axioms.P}⟩
+protected abbrev Hilbert.KP : Hilbert ℕ := ⟨{Axioms.K (.atom 0) (.atom 1), Axioms.P}⟩
+protected abbrev Logic.KP : Logic ℕ := Hilbert.KP.logic
 instance : Hilbert.KP.HasK where p := 0; q := 1
 instance : Hilbert.KP.HasP where
-instance : Entailment.KP (Hilbert.KP) where
+instance : Entailment.KP (Logic.KP) where
 
-open Entailment in
-theorem iff_provable_KP_provable_KD : (Hilbert.KP ⊢! φ) ↔ (Hilbert.KD ⊢! φ) := by
+instance : (Logic.KP) ≊ (Logic.KD) := by
+  apply Entailment.Equiv.antisymm_iff.mpr;
   constructor;
-  . apply fun h ↦ (weakerThan_of_dominate_axioms @h).subset;
-    rintro φ (⟨_, _, rfl⟩ | ⟨_, rfl⟩) <;> simp only [axiomK!, axiomP!];
-  . apply fun h ↦ (weakerThan_of_dominate_axioms @h).subset;
-    rintro φ (⟨_, _, rfl⟩ | (⟨_, rfl⟩)) <;> simp only [axiomK!, axiomD!];
+  . apply Hilbert.weakerThan_of_provable_axioms; rintro φ (rfl | rfl) <;> simp;
+  . apply Hilbert.weakerThan_of_provable_axioms; rintro φ (rfl | rfl) <;> simp;
 
-end LO.Modal.Hilbert
+end LO.Modal
