Foundation/Modal/Logic/Extension.lean
@@ -1,3 +1,4 @@
+import Foundation.Logic.HilbertStyle.Supplemental
 import Foundation.Modal.Logic.Basic
 import Foundation.Modal.Hilbert.K
 
@@ -5,164 +6,108 @@ namespace LO.Modal
 
 open LO.Entailment LO.Modal.Entailment
 
-variable {L L₀ L₁ L₂ L₃ : Logic}
+variable {L L₀ L₁ L₂ L₃ : Logic α}
 
 namespace Logic
 
-protected class IsQuasiNormal (L : Logic) extends Entailment.K L where
-  mdp_closed {φ ψ} : L ⊢! φ ➝ ψ → L ⊢! φ → L ⊢! ψ
-  subst_closed {φ} : L ⊢! φ → ∀ s, L ⊢! φ⟦s⟧
-
-protected class IsNormal (L : Logic) extends L.IsQuasiNormal where
-  nec_closed {φ} : φ ∈ L → □φ ∈ L
-
-
-section
-
-open Entailment
-
-variable [L.IsQuasiNormal]
-variable {φ ψ χ : Formula ℕ}
-
-protected lemma subset_K : Logic.K ⊆ L := IsQuasiNormal.subset_K
-
-protected lemma of_mem_K : φ ∈ Logic.K → φ ∈ L := fun h => Logic.subset_K h
-
-protected lemma mdp (hφψ : φ ➝ ψ ∈ L) (hφ : φ ∈ L) : ψ ∈ L := IsQuasiNormal.mdp_closed hφψ hφ
-
-protected lemma subst (hφ : φ ∈ L) : φ⟦s⟧ ∈ L := IsQuasiNormal.subst_closed hφ s
-
-protected lemma efq (h : ⊥ ∈ L) : ∀ {φ}, φ ∈ L := by
-  intro φ;
-  apply Logic.mdp ?_ h;
-  apply Logic.of_mem_K;
-  simp;
-
-lemma p_q_Apq (hφ : φ ∈ L) (hψ : ψ ∈ L) : φ ⋏ ψ ∈ L := by
-  apply Logic.mdp ?_ hψ;
-  apply Logic.mdp ?_ hφ;
-  apply Logic.of_mem_K;
-  simp;
-
-lemma conj_iffAux {Γ : List (Formula ℕ)} : Γ.conj₂ ∈ L ↔ ∀ φ ∈ Γ, φ ∈ L := by
-  constructor;
-  . intro h φ hφ;
-    refine Logic.mdp ?_ h;
-    apply Logic.of_mem_K;
-    apply left_Conj₂!_intro hφ;
-  . intro h;
-    induction Γ using List.induction_with_singleton with
-    | hnil =>
-      simp only [List.conj₂_nil];
-      apply Logic.of_mem_K;
-      exact verum!;
-    | hsingle φ =>
-      apply h;
-      simp;
-    | @hcons φ Γ hΓ ih =>
-      simp [List.conj₂_cons_nonempty hΓ];
-      apply p_q_Apq;
-      . apply h; tauto;
-      . apply ih; tauto;
-
-lemma conj_iff {Γ : FormulaFinset ℕ} : Γ.conj ∈ L ↔ ∀ φ ∈ Γ, φ ∈ L := by
-  constructor;
-  . intro h φ hφ;
-    apply Logic.conj_iffAux (Γ := Γ.toList) |>.mp $ h;
-    simpa;
-  . intro h;
-    apply Logic.conj_iffAux (Γ := Γ.toList) |>.mpr;
-    intro φ hφ;
-    apply h;
-    simpa using hφ;
-
-section
-
-variable [L.Consistent]
-
-@[simp]
-lemma no_bot : ⊥ ∉ L := by
-  by_contra hC;
-  obtain ⟨φ, hφ⟩ := Set.ne_univ_iff_exists_not_mem L |>.mp $ Consistent.consis;
-  have : φ ∈ L := Logic.efq hC;
-  contradiction;
-
-lemma no_either_no : ¬(φ ∈ L ∧ ∼φ ∈ L) := by
-  rintro ⟨h₁, h₂⟩;
-  exact no_bot $ Logic.mdp h₂ h₁;
-
-lemma not_neg_mem_of_mem : φ ∈ L → ∼φ ∉ L := by
-  have := no_either_no (φ := φ) (L := L);
-  tauto;
-
-lemma not_mem_of_neg_mem : ∼φ ∈ L → φ ∉ L := by
-  have := no_either_no (φ := φ) (L := L);
-  tauto;
-
-end
-
-end
-
-
-section
-
-variable [L.IsNormal]
-
-protected lemma nec (hφ : φ ∈ L) : □φ ∈ L := IsNormal.nec_closed hφ
-
-end
-
-
-inductive sumQuasiNormal (L₁ L₂ : Logic) : Logic
-  | mem₁ {φ}    : φ ∈ L₁ → sumQuasiNormal L₁ L₂ φ
-  | mem₂ {φ}    : φ ∈ L₂ → sumQuasiNormal L₁ L₂ φ
+inductive sumQuasiNormal (L₁ L₂ : Logic α) : Logic α
+  | mem₁ {φ}    : L₁ ⊢! φ → sumQuasiNormal L₁ L₂ φ
+  | mem₂ {φ}    : L₂ ⊢! φ → sumQuasiNormal L₁ L₂ φ
   | mdp  {φ ψ}  : sumQuasiNormal L₁ L₂ (φ ➝ ψ) → sumQuasiNormal L₁ L₂ φ → sumQuasiNormal L₁ L₂ ψ
   | subst {φ s} : sumQuasiNormal L₁ L₂ φ → sumQuasiNormal L₁ L₂ (φ⟦s⟧)
 
-abbrev addQuasiNormal (L : Logic) (φ : Formula ℕ) : Logic := sumQuasiNormal L {φ}
+abbrev addQuasiNormal (L : Logic α) (φ : Formula α) : Logic α := sumQuasiNormal L {φ}
 
-inductive sumNormal (L₁ L₂ : Logic) : Logic
+namespace sumQuasiNormal
+
+variable {φ ψ : Formula α}
+
+lemma mem₁! (hφ : L₁ ⊢! φ) : sumQuasiNormal L₁ L₂ ⊢! φ := by
+  apply iff_provable.mpr;
+  apply sumQuasiNormal.mem₁ hφ;
+
+lemma mem₂! (hφ : L₂ ⊢! φ) : sumQuasiNormal L₁ L₂ ⊢! φ := by
+  apply iff_provable.mpr;
+  apply sumQuasiNormal.mem₂ hφ;
+
+lemma mdp! (hφψ : (sumQuasiNormal L₁ L₂) ⊢! φ ➝ ψ) (hφ : (sumQuasiNormal L₁ L₂) ⊢! φ) : sumQuasiNormal L₁ L₂ ⊢! ψ := by
+  apply iff_provable.mpr;
+  apply sumQuasiNormal.mdp;
+  . apply iff_provable.mp; exact hφψ;
+  . apply iff_provable.mp; exact hφ;
+
+
+lemma symm : sumQuasiNormal L₁ L₂ = sumQuasiNormal L₂ L₁ := by
+  ext φ;
+  constructor;
+  . intro h;
+    induction h with
+    | mem₁ h => exact sumQuasiNormal.mem₂ h;
+    | mem₂ h => exact sumQuasiNormal.mem₁ h;
+    | mdp _ _ ihφψ ihφ => exact sumQuasiNormal.mdp ihφψ ihφ;
+    | subst _ ihφ => exact sumQuasiNormal.subst ihφ;
+  . intro h;
+    induction h with
+    | mem₁ h => exact sumQuasiNormal.mem₂ h;
+    | mem₂ h => exact sumQuasiNormal.mem₁ h;
+    | mdp _ _ ihφψ ihφ => exact sumQuasiNormal.mdp ihφψ ihφ;
+    | subst _ ihφ => exact sumQuasiNormal.subst ihφ;
+
+variable [DecidableEq α]
+
+instance [L₁.IsQuasiNormal] : Entailment.Lukasiewicz (sumQuasiNormal L₁ L₂) where
+  imply₁ _ _ := by constructor; apply sumQuasiNormal.mem₁; simp;
+  imply₂ _ _ _ := by constructor; apply sumQuasiNormal.mem₁; simp;
+  elimContra _ _ := by constructor; apply sumQuasiNormal.mem₁; simp;
+  mdp hφψ hφ := by
+    constructor;
+    apply sumQuasiNormal.mdp;
+    . exact PLift.down hφψ;
+    . exact PLift.down hφ;
+
+instance [L₁.IsQuasiNormal] : (sumQuasiNormal L₁ L₂).IsQuasiNormal where
+  K _ _ := by constructor; apply sumQuasiNormal.mem₁; simp;
+  subst s hφ := by
+    constructor;
+    apply sumQuasiNormal.subst;
+    exact PLift.down hφ;
+
+instance [L₂.IsQuasiNormal] : (sumQuasiNormal L₁ L₂).IsQuasiNormal := by
+  rw [sumQuasiNormal.symm];
+  infer_instance;
+
+instance : L₁ ⪯ sumQuasiNormal L₁ L₂ := by
+  apply weakerThan_iff.mpr;
+  intro φ hφ;
+  apply iff_provable.mpr;
+  apply sumQuasiNormal.mem₁ hφ;
+
+instance : L₂ ⪯ sumQuasiNormal L₁ L₂ := by
+  rw [sumQuasiNormal.symm];
+  infer_instance;
+
+end sumQuasiNormal
+
+
+inductive sumNormal (L₁ L₂ : Logic α) : Logic α
   | mem₁ {φ}    : φ ∈ L₁ → sumNormal L₁ L₂ φ
   | mem₂ {φ}    : φ ∈ L₂ → sumNormal L₁ L₂ φ
   | mdp  {φ ψ}  : sumNormal L₁ L₂ (φ ➝ ψ) → sumNormal L₁ L₂ φ → sumNormal L₁ L₂ ψ
   | subst {φ s} : sumNormal L₁ L₂ φ → sumNormal L₁ L₂ (φ⟦s⟧)
   | nec {φ}     : sumNormal L₁ L₂ φ → sumNormal L₁ L₂ (□φ)
 
-abbrev addNormal (L : Logic) (φ : Formula ℕ) : Logic := sumNormal L {φ}
+abbrev addNormal (L : Logic α) (φ : Formula α) : Logic α := sumNormal L {φ}
+
+namespace sumNormal
+
+end sumNormal
 
 end Logic
 
 
 
-namespace Hilbert
 
-open Entailment
-
-instance {H : Hilbert ℕ} [H.HasK] : (H.logic).IsNormal where
-  /-
-  subset_K := by
-    intro φ hφ;
-    induction hφ using Hilbert.Deduction.rec! with
-    | maxm h =>
-      rcases (by simpa using h) with ⟨s, rfl⟩; simp;
-    | mdp ihφψ ihφ => exact mdp! ihφψ ihφ;
-    | nec ih => exact nec! ih;
-    | _ => simp;
-  -/
-  mdp_closed := by
-    intro φ ψ hφψ hφ;
-    exact hφψ ⨀ hφ;
-  subst_closed := by
-    intro φ hφ s;
-    exact Hilbert.Deduction.subst! s hφ;
-  nec_closed := by
-    intro φ hφ;
-    exact Entailment.nec! hφ;
-
-end Hilbert
-
-
-
+/-
 def QuasiNormalExtension (L : Logic) := { L' : Logic // L ⊆ L' ∧ L'.IsQuasiNormal }
 
 namespace QuasiNormalExtension
@@ -242,5 +187,6 @@ def ExtensionNormal (L : Logic) := { L' : Logic // L'.IsNormal ∧ L ⊆ L' }
 namespace ExtensionNormal
 
 end ExtensionNormal
+-/
 
 end LO.Modal
