Foundation/Modal/Kripke/Logic/Ver.lean
@@ -4,9 +4,12 @@ import Foundation.Modal.Kripke.Logic.KTc
 
 namespace LO.Modal
 
-open Kripke
+open Entailment
+open Entailment.Context
+open Formula
+open Formula.Kripke
 open Hilbert.Kripke
-
+open Kripke
 
 namespace Kripke
 
@@ -27,7 +30,7 @@ end Kripke
 
 namespace Logic.Ver.Kripke
 
-instance : Sound Hilbert.Ver FrameClass.Ver := instSound_of_validates_axioms $ by
+instance : Sound Logic.Ver FrameClass.Ver := instSound_of_validates_axioms $ by
   apply FrameClass.Validates.withAxiomK;
   rintro F hF _ (rfl | rfl);
   simp_all only [Set.mem_setOf_eq];
@@ -52,9 +55,9 @@ instance : Kripke.Canonical Logic.Ver FrameClass.Ver := ⟨by
 
 instance : Complete Logic.Ver FrameClass.Ver := inferInstance
 
-instance : Complete (Logic.Ver) Kripke.FrameClass.finite_Ver := ⟨by
+instance complete : Complete (Logic.Ver) Kripke.FrameClass.finite_Ver := ⟨by
   intro φ hφ;
-  apply LO.Complete.complete (𝓢 := Hilbert.Ver) (𝓜 := FrameClass.Ver);
+  apply LO.Complete.complete (𝓢 := Logic.Ver) (𝓜 := FrameClass.Ver);
   intro F hF V r;
   apply Model.pointGenerate.modal_equivalent_at_root (r := r) |>.mp;
   apply hφ;
@@ -79,36 +82,40 @@ lemma finite_Ver : Logic.Ver = FrameClass.finite_Ver.logic := eq_hilbert_logic_f
 
 instance : Logic.KTc ⪱ Logic.Ver := by
   constructor;
-  . rw [KTc.Kripke.corefl, Ver.Kripke.isolated];
+  . apply Entailment.weakerThan_iff.mpr;
+    suffices ∀ φ, FrameClass.KTc ⊧ φ → FrameClass.Ver ⊧ φ by
+      simpa [KTc.Kripke.corefl, Ver.Kripke.isolated];
     rintro φ hφ F hF;
     replace hF := Set.mem_setOf_eq.mp hF;
     apply hφ;
     apply Set.mem_setOf_eq.mpr;
     infer_instance;
-  . suffices ∃ φ, Hilbert.Ver ⊢! φ ∧ ¬FrameClass.KTc ⊧ φ by
-      rw [KTc.Kripke.corefl];
-      tauto;
+  . apply Entailment.not_weakerThan_iff.mpr;
+    suffices ∃ φ, Logic.Ver ⊢! φ ∧ ¬FrameClass.KTc ⊧ φ by simpa [KTc.Kripke.corefl];
     use (Axioms.Ver ⊥);
     constructor;
-    . exact axiomVer!;
+    . simp;
     . apply Kripke.not_validOnFrameClass_of_exists_model_world;
       let M : Model := ⟨⟨Fin 1, λ x y => True⟩, λ w _ => False⟩;
       use M, 0;
       constructor;
       . refine ⟨by unfold Coreflexive; trivial⟩
-      . suffices ∃ x, (0 : M.World) ≺ x by simpa [Satisfies, Semantics.Realize];
+      . suffices ∃ x, (0 : M.World) ≺ x by
+          simpa [Satisfies, Semantics.Realize];
         use 0;
 
 instance : Logic.GLPoint3 ⪱ Logic.Ver := by
   constructor;
-  . rw [GLPoint3.Kripke.finite_strict_linear_order, Ver.Kripke.finite_Ver];
+  . apply Entailment.weakerThan_iff.mpr;
+    suffices ∀ φ, FrameClass.finite_GLPoint3 ⊧ φ → FrameClass.finite_Ver ⊧ φ by
+      simpa [GLPoint3.Kripke.finite_strict_linear_order, Ver.Kripke.finite_Ver];
     rintro φ hφ F hF;
+    replace hF := Set.mem_setOf_eq.mp hF;
     apply hφ;
-    simp_all only [Set.mem_setOf_eq];
+    apply Set.mem_setOf_eq.mpr;
     infer_instance;
-  . suffices ∃ φ, Hilbert.Ver ⊢! φ ∧ ¬FrameClass.finite_GLPoint3 ⊧ φ by
-      rw [GLPoint3.Kripke.finite_strict_linear_order];
-      tauto;
+  . apply Entailment.not_weakerThan_iff.mpr;
+    suffices ∃ φ, Logic.Ver ⊢! φ ∧ ¬FrameClass.finite_GLPoint3 ⊧ φ by simpa [GLPoint3.Kripke.finite_strict_linear_order];
     use (Axioms.Ver ⊥);
     constructor;
     . simp;
@@ -120,8 +127,6 @@ instance : Logic.GLPoint3 ⪱ Logic.Ver := by
         use 1;
         tauto;
 
-instance : Logic.Ver ⪱ Logic.Univ := by  constructor <;> simp;
-
-end Logic
+end Logic.Ver.Kripke
 
 end LO.Modal
