Foundation/Modal/Logic/S/Basic.lean
@@ -6,41 +6,26 @@ namespace LO.Modal
 open Logic
 
 protected abbrev Logic.S := addQuasiNormal Logic.GL (Axioms.T (.atom 0))
-instance : Logic.S.IsQuasiNormal where
-  subset_K := by
-    intro φ hφ;
-    apply Logic.sumQuasiNormal.mem₁;
-    exact Logic.of_mem_K hφ;
-  mdp_closed := by
-    intro φ ψ hφψ hφ;
-    apply Logic.sumQuasiNormal.mdp hφψ hφ;
-  subst_closed := by
-    intro φ hφ s;
-    apply Logic.sumQuasiNormal.subst;
-    exact hφ;
+instance : Logic.S.IsQuasiNormal := inferInstance
+instance : Entailment.HasAxiomT Logic.S where
+  T φ := by
+    constructor;
+    apply Logic.sumQuasiNormal.subst (φ := Axioms.T (.atom 0)) (s := λ _ => φ);
+    apply Logic.sumQuasiNormal.mem₂;
+    simp;
 
-lemma Logic.S.mem_axiomT : □φ ➝ φ ∈ Logic.S := by
-  apply Logic.subst (φ := Axioms.T (.atom 0)) (s := λ _ => φ);
-  apply Logic.sumQuasiNormal.mem₂;
-  tauto;
-
-lemma Logic.GL_subset_S : Logic.GL ⊆ Logic.S := by
-  intro φ hφ;
-  apply Logic.sumQuasiNormal.mem₁;
-  assumption;
-
-lemma Logic.GL_ssubset_S : Logic.GL ⪱ Logic.S := by
+instance : Logic.GL ⪱ Logic.S := by
   constructor;
-  . exact Logic.GL_subset_S;
-  . suffices ∃ φ, φ ∈ Logic.S ∧ φ ∉ Logic.GL by exact Set.not_subset.mpr this;
+  . infer_instance;
+  . apply Entailment.not_weakerThan_iff.mpr;
     use (Axioms.T (.atom 0));
     constructor;
-    . exact Logic.S.mem_axiomT;
+    . simp;
     . exact Logic.GL.unprovable_AxiomT;
-
 
 section
 
+/-
 private inductive Logic.S' : Logic
   | mem_GL {φ} : φ ∈ Logic.GL → Logic.S' φ
   | axiomT (φ) : Logic.S' (Axioms.T φ)
@@ -71,16 +56,32 @@ private lemma Logic.eq_S_S' : Logic.S = Logic.S' := by
       exact sumQuasiNormal.subst (φ := Axioms.T (.atom 0)) (s := λ _ => φ) $ by
         apply Logic.sumQuasiNormal.mem₂;
         simp;
+-/
 
 -- TODO: Remove `eq_S_S'`?
 protected def Logic.S.rec'
-  {motive : (φ : Formula ℕ) → φ ∈ Logic.S → Prop}
-  (mem_GL : ∀ {φ}, (h : φ ∈ Logic.GL) → motive φ (sumQuasiNormal.mem₁ h))
-  (axiomT : ∀ {φ}, motive (Axioms.T φ) (sumQuasiNormal.subst (φ := Axioms.T (.atom 0)) (s := λ _ => φ) (sumQuasiNormal.mem₂ (by tauto))))
-  (mdp : ∀ {φ ψ}, {hφψ : φ ➝ ψ ∈ Logic.S} → {hφ : φ ∈ Logic.S} → (motive (φ ➝ ψ) hφψ) → (motive φ hφ) → motive ψ (sumQuasiNormal.mdp hφψ hφ))
-  : ∀ {φ}, (h : φ ∈ Logic.S) → motive φ h := by
+  {motive : (φ : Formula ℕ) → (Logic.S ⊢! φ) → Prop}
+  (mem_GL : ∀ {φ}, (h : Logic.GL ⊢! φ) → motive φ (sumQuasiNormal.mem₁! h))
+  (axiomT : ∀ {φ}, motive (Axioms.T φ) (by simp))
+  (mdp : ∀ {φ ψ}, {hφψ : Logic.S ⊢! φ ➝ ψ} → {hφ : Logic.S ⊢! φ} → (motive (φ ➝ ψ) hφψ) → (motive φ hφ) → motive ψ (sumQuasiNormal.mdp! hφψ hφ))
+  : ∀ {φ}, (h : Logic.S ⊢! φ) → motive φ h := by
   intro φ h;
-  rw [Logic.eq_S_S'] at h;
+  induction (iff_provable.mp h) with
+  | mem₁ h₁ => apply mem_GL; assumption;
+  | mem₂ h₂ =>
+    replace h₂ := iff_provable.mp h₂; subst h₂;
+    apply axiomT;
+  | mdp hφψ hφ ihφψ ihφ =>
+    apply mdp;
+    . apply ihφψ;
+    . apply ihφ;
+    . apply iff_provable.mpr; exact hφψ;
+    . apply iff_provable.mpr; exact hφ;
+  | @subst φ s hφ ihφ =>
+    generalize φ⟦s⟧ = ψ at h ⊢;
+    sorry;
+
+  /-
   induction h with
   | mem_GL h => apply mem_GL; assumption;
   | axiomT h => exact axiomT;
@@ -90,6 +91,7 @@ protected def Logic.S.rec'
     . apply ihφ;
     . rwa [←Logic.eq_S_S'] at hφψ;
     . rwa [←Logic.eq_S_S'] at hφ;
+-/
 
 end
 
